Sort.v
@@ -1,0 +1,277 @@
+Load List.
+
+Class DecidableBinaryRelation {A} (r : A -> A -> Prop) := {
+  decide_binary_relation : A -> A -> bool;
+  DecidableBinaryRelation_spec : forall a b, reflect (r a b) (decide_binary_relation a b);
+}.
+
+Class TotalOrder {A} (r : A -> A -> Prop) := {
+  TotalOrder_DecidableBinaryRelation :> DecidableBinaryRelation r;
+  TotalOrder_reflexivity : forall a, r a a;
+  TotalOrder_transitivity : forall a b c, r a b -> r b c -> r a c;
+  TotalOrder_antisymmetry : forall a b, r a b -> r b a -> a = b;
+  TotalOrder_totality : forall a b, r a b \/ r b a;
+}.
+
+Coercion TotalOrder_DecidableBinaryRelation : TotalOrder >-> DecidableBinaryRelation.
+
+Class CostTotalOrder {A} (r : A -> A -> Prop) := {
+  CostTotalOrder_TotalOrder :> TotalOrder r;
+  CostTotalOrder_cost : Cost (Signature [_; _] _) decide_binary_relation;
+}.
+
+Coercion CostTotalOrder_TotalOrder : CostTotalOrder >-> TotalOrder.
+
+Class CostConstantTotalOrder {A} (r : A -> A -> Prop) := {
+  CostConstantTotalOrder_CostTotalOrder :> CostTotalOrder r;
+  CostConstantTotalOrder_cost_constant : binary_cost_constant CostTotalOrder_cost;
+}.
+
+Coercion CostConstantTotalOrder_CostTotalOrder : CostConstantTotalOrder >-> CostTotalOrder.
+
+#[export, program] Instance nat_le_DecidableBinaryRelation : DecidableBinaryRelation Nat.le := {
+  decide_binary_relation := Nat.leb;
+}.
+Next Obligation.
+  apply Nat.leb_spec0.
+Qed.
+
+#[export, program] Instance nat_le_TotalOrder : TotalOrder Nat.le.
+Next Obligation.
+  lia.
+Qed.
+Next Obligation.
+  lia.
+Qed.
+Next Obligation.
+  lia.
+Qed.
+
+#[export, program] Instance nat_leb_Cost : Cost (Signature [_; _] _) Nat.leb := {
+  cost_fun := fun _ _ => 1;
+}.
+
+#[export, program] Instance nat_le_CostTotalOrder : CostTotalOrder Nat.le.
+
+#[export, program] Instance nat_le_CostConstantTotalOrder : CostConstantTotalOrder Nat.le.
+Next Obligation.
+  exists 1. intros ?. simpl. destruct a. lia.
+Qed.
+
+Fixpoint sorted {A} r {total_order : TotalOrder r} (l : list A) :=
+  match l with
+  | [] => True
+  | x :: l' => (list_forall (fun y => r x y) l') /\ sorted r l'
+  end.
+
+Fixpoint simple_sorted {A} r {total_order : TotalOrder r} (l : list A) :=
+  match l with
+  | [] => True
+  | [_] => True
+  | x :: ((y :: _) as l') => r x y /\ simple_sorted r l'
+  end.
+
+Theorem simple_sorted_iff_sorted :
+  forall {A} r {total_order : TotalOrder r} (l : list A),
+  simple_sorted r l <-> sorted r l.
+Proof.
+  intros ? ? ? ?. induction l.
+  - simpl. intuition auto.
+  - simpl. destruct l.
+    + simpl. intuition auto.
+    + rename a0 into b.
+      remember (simple_sorted r (b :: l)) as P. simpl. subst P.
+      split.
+      * intros (? & ?). specialize (proj1 IHl H0) as (? & ?). repeat split.
+        -- auto.
+        -- eapply list_forall_positive.
+           2: apply H1.
+           eauto using TotalOrder_transitivity.
+        -- auto.
+        -- auto.
+      * intros ((? & ?) & ? & ?). split.
+        -- auto.
+        -- apply IHl. simpl. auto.
+Qed.
+
+Definition simple_sortedb {A} r {total_order : TotalOrder r} :=
+  fix simple_sortedb (l : list A) :=
+    match l with
+    | [] => true
+    | [_] => true
+    | x :: ((y :: _) as l') => (@decide_binary_relation _ r _) x y && simple_sortedb l'
+    end.
+
+Theorem simple_sortedb_spec :
+  forall {A} r {total_order : TotalOrder r} (l : list A),
+  reflect (simple_sorted r l) (simple_sortedb r l).
+Proof.
+  intros ? ? ? ?. induction l.
+  - simpl. apply ReflectT. auto.
+  - simpl. destruct l.
+    + apply ReflectT. auto.
+    + rename a0 into b.
+      destruct (@DecidableBinaryRelation_spec _ r _ a b); destruct IHl; constructor; intuition auto.
+Qed.
+
+Definition simple_sortedb_cost {A} r {total_order : CostTotalOrder r} :=
+  ltac2:(
+    Cost.refine_compute_cost
+    [
+      (
+        ('(@decide_binary_relation _ _ total_order), 2),
+        '(@cost_fun _ _ (@CostTotalOrder_cost _ _ total_order))
+      )
+    ]
+    1
+    (eval red in (@simple_sortedb A r total_order))
+    []
+  ).
+
+Theorem simple_sortedb_cost_linear_on_cost_constant_total_order :
+  forall {A} r {total_order : CostConstantTotalOrder r},
+  big_o
+    (simple_sortedb_cost r)
+    (fun (l : list A) => 1 + length l).
+Proof.
+  intros ? ? ?. destruct total_order as (total_order & (c & H)). exists (c + 18). intros l. induction l.
+  - simpl. lia.
+  - simpl. destruct l.
+    + lia.
+    + rename a0 into b. unfold CostConstantTotalOrder_CostTotalOrder in IHl.
+      specialize (H (a, b)). simpl in H. lia.
+Qed.
+
+Definition is_sorter {A} r {total_order : TotalOrder r} f :=
+  forall (l : list A), is_permutation (f l) l /\ sorted r (f l).
+
+Definition insert_sorted {A} r {total_order : TotalOrder r} :=
+  fix insert_sorted a (l : list A) :=
+    match l with
+    | [] => [a]
+    | x :: l' =>
+      if (@decide_binary_relation _ r _) a x
+      then a :: x :: l'
+      else x :: (insert_sorted a l')
+    end.
+
+Theorem insert_sorted_correct :
+  forall {A} r {total_order : TotalOrder r} a (l : list A),
+  sorted r l ->
+  is_permutation (insert_sorted r a l) (a :: l) /\ sorted r (insert_sorted r a l).
+Proof.
+  intros ? ? ? ? ? ?. induction l.
+  - simpl. split.
+    + apply is_permutation_add. apply is_permutation_empty.
+    + auto.
+  - rename a0 into b. destruct H as (? & ?). apply IHl in H0 as ?. destruct H1 as (? & ?).
+    simpl. destruct (@DecidableBinaryRelation_spec _ r _ a b).
+    + split.
+      * apply is_permutation_refl.
+      * simpl. repeat split.
+        -- auto.
+        -- eapply list_forall_positive.
+           2: apply H.
+           eauto using TotalOrder_transitivity.
+        -- auto.
+        -- auto.
+    + split.
+      * apply is_permutation_trans with (b :: a :: l).
+        -- apply is_permutation_add. auto.
+        -- apply is_permutation_swap.
+      * simpl. split.
+        -- apply list_forall_permutation with (a :: l).
+           ++ apply is_permutation_sym. auto.
+           ++ simpl. split.
+              ** destruct (@TotalOrder_totality _ r _ a b); intuition auto.
+              ** auto.
+        -- auto.
+Qed.
+
+Definition insert_sorted_cost {A} r {total_order : CostTotalOrder r} :=
+  ltac2:(
+    Cost.refine_compute_cost
+    [
+      (
+        ('(@decide_binary_relation _ _ total_order), 2),
+        '(@cost_fun _ _ (@CostTotalOrder_cost _ _ total_order))
+      )
+    ]
+    2
+    (eval red in (@insert_sorted A r total_order))
+    []
+  ).
+
+Theorem insert_sorted_cost_linear_on_cost_constant_total_order :
+  forall {A} r {total_order : CostConstantTotalOrder r},
+  big_o
+    (fun '(a, l) => insert_sorted_cost r a l)
+    (fun '(_, l) => 1 + length (l : list A)).
+Proof.
+  intros ? ? ?. destruct total_order as (total_order & (c & H)). exists (c + 19). intros (a, l). induction l.
+  - simpl. lia.
+  - rename a0 into b. unfold CostConstantTotalOrder_CostTotalOrder in IHl. simpl. specialize (H (a, b)).
+    destruct (@DecidableBinaryRelation_spec _ r _ a b); lia.
+Qed.
+
+Definition insertion_sort {A} r {total_order : TotalOrder r} :=
+  fix insertion_sort (l : list A) :=
+    match l with
+    | [] => []
+    | x :: l' => insert_sorted r x (insertion_sort l')
+    end.
+
+Theorem insertion_sort_correct :
+  forall {A} (r : A -> A -> Prop) {total_order : TotalOrder r}, is_sorter r (insertion_sort r).
+Proof.
+  unfold is_sorter. intros ? ? ? ?. induction l.
+  - simpl. auto using is_permutation_empty.
+  - simpl. destruct IHl as (IHl1 & IHl2).
+    specialize (insert_sorted_correct r a (insertion_sort r l) IHl2) as (? & ?).
+    split.
+    + apply is_permutation_trans with (a :: (insertion_sort r l)).
+      * auto.
+      * apply is_permutation_add. auto.
+    + auto.
+Qed.
+
+Definition insertion_sort_cost {A} r {total_order : CostTotalOrder r} :=
+  ltac2:(
+    Cost.refine_compute_cost
+    [
+      (
+        ('(@insert_sorted A r total_order), 2),
+        '(@insert_sorted_cost A r total_order)
+      )
+    ]
+    1
+    (eval red in (@insertion_sort A r total_order))
+    ['(@insertion_sort A r total_order)]
+  ).
+
+Theorem insertion_sort_cost_quadratic_on_cost_constant_total_order :
+  forall {A} r {total_order : CostConstantTotalOrder r},
+  big_o
+    (insertion_sort_cost r)
+    (fun (l : list A) => 1 + (length l) * (length l)).
+Proof.
+  intros ? ? ?. destruct (insert_sorted_cost_linear_on_cost_constant_total_order r) as (c & H).
+  exists (c + 10). intros l. induction l.
+  - simpl. lia.
+  - simpl.
+    specialize (H (a, insertion_sort r l)). simpl in H.
+    replace (length (insertion_sort r l))
+      with (length l)
+      in H
+      by (apply permutation_length; apply insertion_sort_correct).
+    lia.
+Qed.
+
+Section Example.
+
+Compute insertion_sort_cost _ [1; 1; 1; 1; 1; 1; 1; 1; 1; 1; 1; 1; 1; 1; 1; 1].
+Compute insertion_sort_cost _ [1; 2; 3; 4; 5; 6; 7; 8; 9; 10].
+Compute insertion_sort_cost _ [10; 9; 8; 7; 6; 5; 4; 3; 2; 1].
+Compute insertion_sort_cost _ [20; 19; 18; 17; 16; 15; 14; 13; 12; 11; 10; 9; 8; 7; 6; 5; 4; 3; 2; 1].
+
+End Example.
